theories/soundness/expr.v
@@ -26,6 +26,8 @@ Section proofs.
   Lemma expr_soundness (Δ: list constraint) rigid (Σ: list (interp Θ)) kd e Γ Ω ty val :
     map_Forall (λ _, wf_cdef_parent pdefs) pdefs →
     map_Forall (λ _, wf_cdef_mono) pdefs →
+    map_Forall (λ _ : string, wf_cdef_constraints_wf) pdefs →
+    map_Forall (λ _ : string, wf_cdef_constraints_bounded) pdefs →
     Forall wf_constraint Δ →
     wf_lty Γ →
     expr_eval Ω e = Some val →
@@ -35,7 +37,7 @@ Section proofs.
     interp_local_tys Σ Γ Ω -∗
     interp_type ty Σ val.
   Proof.
-    move => ??? wflty he h; move: Ω val he.
+    move => ????? wflty he h; move: Ω val he.
     induction h as [| | | kd op e1 e2 hop he1 hi1 he2 hi2 |
         kd op e1 e2 hop he1 hi1 he2 hi2 | kd e1 e2 h1 hi1 h2 hi2 | kd e0 h hi |
         kd v vty hv | | kd exp S T hS hi hwf hok hsub | kd exp S T hS hi hwf hok hsub]
